ITree.lean
@@ -2,3 +2,4 @@ import ITree.Definition
 import ITree.Effect
 import ITree.Effects
 import ITree.Exec
+import ITree.Eval
