ITree/Effects.lean
@@ -2,4 +2,5 @@ import ITree.Effects.Conc
 import ITree.Effects.Demonic
 import ITree.Effects.Fail
 import ITree.Effects.Heap
+import ITree.Effects.Log
 import ITree.Effects.State
