ITree/Effects/Heap.lean
@@ -45,14 +45,27 @@ def HeapE.load! [heapE Loc Val -< E] [failE -< E] (l : Loc) : ITree E Val := do
   return v
 export HeapE (load!)
 
-def HeapE.allocN [heapE Loc Val -< E] [demonicE (List Loc) -< E] (P : List Loc → Prop) (v : Val) : ITree E {ls // P ls} := do
+/- TODO: can we make this an instance? -/
+def inhabited_free_locs {n} (hmap : heapE.T Loc Val) [Zero Loc] [HAdd Loc Int Loc] [Std.LawfulEqOrd Loc] (hlt : ∀ (l : Loc) (m : Nat), ¬(compare (l + (1 : Int) + (m : Int)) l).isLE) : Inhabited { l // ∀ (m : Nat), m < n → (l : Loc) + (m : Int) ∉ hmap } where
+  default := ⟨match hmap.maxKey? with | some n => n + (1 : Int) | none => 0, by
+    intro m hm
+    cases h : (hmap.maxKey?) <;>
+      simp [hmap.maxKey?_eq_none_iff,
+        hmap.maxKey?_eq_some_iff_mem_and_forall] at h <;> simp [h]
+    next max =>
+    have ⟨_, h⟩ := h;
+    intros contra
+    replace contra := h _ contra
+    grind
+  ⟩
+
+def HeapE.allocN [heapE Loc Val -< E] [demonicE Loc -< E] [Zero Loc] [HAdd Loc Int Loc] [Std.LawfulEqOrd Loc] (n : Nat) (v : Val) (hle : ∀ (l : Loc) (m : Nat), ¬(compare (l + (1 : Int) + (m : Int)) l).isLE = true) : ITree E Loc := do
   let hmap ← get
-  let ⟨ls, _⟩ ← choose (λ ls : List _ => P ls ∧ ∀ l ∈ ls, l ∉ hmap)
-  set (hmap.insertMany $ ls.map λ l => ⟨l, some v⟩)
-  return ⟨ls, by grind⟩
+  let ⟨l, _⟩ ← choose (hi := inhabited_free_locs hmap hle) (λ l : Loc => ∀ m : Nat, m < n → l + (m : Int) ∉ hmap)
+  set (hmap.insertMany $ (List.range n).map λ m => ⟨l + (m : Int), some v⟩)
+  return l
 export HeapE (allocN)
 
-def HeapE.alloc [heapE Loc Val -< E] [demonicE (List Loc) -< E] (v : Val) : ITree E Loc := do
-  let ⟨ls, _⟩ ← allocN (·.length = 1) v
-  return ls.head (by grind)
+def HeapE.alloc [heapE Loc Val -< E] [demonicE Loc -< E] [Zero Loc] [HAdd Loc Int Loc] [Std.LawfulEqOrd Loc]
+  (v : Val) (hle : ∀ (l : Loc) (m : Nat), ¬(compare (l + (1 : Int) + (m : Int)) l).isLE = true) : ITree E Loc := allocN 1 v hle
 export HeapE (alloc)
