ITree/Effects/Log.lean
@@ -1,0 +1,24 @@
+import Lean.Log
+import ITree.Effect
+import ITree.Definition
+import ITree.Exec
+import ITree.Eval
+
+namespace ITree.Effects
+open Lean
+
+def logE (α : Type u) : Effect.{u} where
+  I := α
+  O _ := PUnit
+
+def LogE.log {α : Type u} {E} [logE α -< E] (a : α) : ITree.{u} E PUnit :=
+  .trigger (logE α) (a)
+export LogE (log)
+
+section Eval
+open ITree.Eval
+
+instance logMH {α m} [Monad m] [MonadLog m] [AddMessageContext m] [MonadOptions m] [ToMessageData α] : SMHandler (logE α) m where
+  handle i := let i : α := i; logInfo m!"{i}"
+
+end Eval
