ITree/Eval.lean
@@ -1,0 +1,42 @@
+import ITree.Definition
+
+namespace ITree.Eval
+
+class MHandler (E : Effect.{u}) (T : Type u) (m : Type u → Type u) [Monad m] where
+  handle : (i : E.I) → (k : E.O i → T) → m T
+
+class SMHandler (E : Effect.{u}) (m : Type u → Type u) [Monad m] where
+  handle : (i : E.I) → m (E.O i)
+
+instance SMHandler.toMHandler {E : Effect.{u}} {T : Type u} {m : Type u → Type u} [Monad m] [SMHandler E m]
+    : MHandler E T m where
+  handle i k := SMHandler.handle i >>= (pure $ k ·)
+
+/- TODO: Should we require a MonoBind instance and define this using partial fixpoint? This would allow us to prove stuff about this definition. -/
+partial def eval {GE : Effect.{u}} {GR : Type u} (m : Type u → Type u) [Monad m] [MHandler GE (ITree GE GR) m] [Inhabited GR] (t : ITree GE GR) : m GR :=
+  match t.unfold with
+  | .ret r => return r
+  | .tau t => eval m t
+  | .vis i k => MHandler.handle i k >>= eval m
+
+partial def evalNGo {GE : Effect.{u}} {GR : Type u} (m : Type u → Type u) [Monad m] [mh : MHandler GE ((n : Nat) × (ITreeN GE GR n)) m] :
+  (n : Nat) → (Coinductive.CoIndN (ITreeF GE GR) n) → m (Option GR)
+  | 0, _ => return none
+  | _+1, .ret r => return some r
+  | n+1, .tau t => evalNGo m n t
+  | _+1, .vis i k => mh.handle i (λ o => ⟨_, k o⟩) >>=
+    λ o => let ⟨n, t⟩ := o; evalNGo m n t
+
+def evalN {GE : Effect.{u}} {GR : Type u} (m : Type u → Type u) [Monad m] [MHandler GE ((n : Nat) × (ITreeN GE GR n)) m] (n : Nat) (t : ITree GE GR) : m (Option GR) := evalNGo m n (t.approx n)
+
+instance sumMH {E₁ E₂ : Effect.{u}} {m T} [Monad m] [mh₁ : MHandler E₁ T m] [mh₂ : MHandler E₂ T m]
+    : MHandler (E₁ ⊕ₑ E₂) T m where
+  handle i k := match i with
+    | .inl i => MHandler.handle i k
+    | .inr i => MHandler.handle i k
+
+instance sumSMH {E₁ E₂ : Effect} {m} [Monad m] [mh₁ : SMHandler E₁ m] [mh₂ : SMHandler E₂ m]
+    : SMHandler (E₁ ⊕ₑ E₂) m where
+  handle i := match i with
+    | .inl i => mh₁.handle i
+    | .inr i => mh₂.handle i
