Test/ITreeEval.lean
@@ -1,0 +1,127 @@
+import Lean
+import ITree
+
+namespace Test
+open ITree ITree.Effects ITree.Eval
+
+def add_1_plus_1 : ITree failE Nat := do
+  let x ← (pure 1);
+  return x + 1
+
+def add_1_plus_1_fail : ITree failE Nat := do
+  let x ← (pure 1);
+  fail s!"result: {x + 1}"
+
+/-- info: Except.ok 2 -/
+#guard_msgs in
+#eval eval (Except String) add_1_plus_1
+
+/-- info: Except.error "result: 2" -/
+#guard_msgs in
+#eval eval (Except String) add_1_plus_1_fail
+
+local instance : MonadEval (ExceptT String Lean.Elab.Command.CommandElabM) Lean.Elab.Command.CommandElabM where
+  monadEval x := do
+    let r ← x
+    match r with
+    | .ok v => return v
+    | .error msg => throw (Lean.Exception.error .missing s!"Evaluation failed with message: {msg}")
+
+/-- error: Evaluation failed with message: result: 2 -/
+#guard_msgs in
+#eval eval (ExceptT String Lean.Elab.Command.CommandElabM) add_1_plus_1_fail
+
+def print : Nat → ITree (logE Nat) Nat
+  | 0 => return 0
+  | n+1 => do log n; print n
+
+/--
+info: 9
+---
+info: 8
+---
+info: 7
+---
+info: 6
+---
+info: 5
+---
+info: 4
+---
+info: 3
+---
+info: 2
+---
+info: 1
+---
+info: 0
+---
+info: some 0
+-/
+#guard_msgs in
+#eval evalN (Lean.Elab.Command.CommandElabM) 20000 (print 10)
+
+def test_state : ITree (stateE Nat ⊕ₑ failE) Nat := do
+  set 0;
+  let x ← get;
+  assert (x = 0)
+  return x
+
+local instance : MonadEval (StateT Nat (Except String)) IO where
+  monadEval x := do
+    let r := x.run 0
+    match r with
+    | .ok v => return v.1
+    | .error msg => IO.ofExcept $ .error (s!"Evaluation failed: {msg}")
+
+/-- info: some 0 -/
+#guard_msgs in
+#eval evalN (StateT Nat (Except String)) 20000 (test_state)
+
+abbrev raceE := stateE Nat ⊕ₑ concE ⊕ₑ failE
+
+abbrev raceM := StateT (ConcState ((n : Nat) × ITreeN raceE Nat n)) (StateT Nat (Except String))
+
+local instance : MonadEval raceM IO where
+  monadEval x := do
+    let r := (x.run (ConcState.new)).run 0
+    match r with
+    | .ok v => return v.1.1
+    | .error msg => IO.ofExcept $ .error (s!"Evaluation failed: {msg}")
+
+def test_race : ITree raceE Nat := do
+  set 0;
+  fork (do let x ← get; yield; set (x + 1); yield)
+  let x ← get; yield; set (x + 1); yield;
+
+  let x' ← get; yield; assert (x' = 2); yield;
+  return x'
+
+def test_race_ok : ITree (stateE Nat ⊕ₑ concE ⊕ₑ failE) Nat := do
+  set 0;
+  fork (do let x ← get; yield; set (x + 1); yield)
+  let x ← get; yield; set (x + 1); yield;
+
+  let x' ← get; yield; assert (x' = 1); yield;
+  return x'
+
+def test_race_ok2 : ITree (stateE Nat ⊕ₑ concE ⊕ₑ failE) Nat := do
+  set 0;
+  fork (do let x ← get; yield; set (x + 1); yield)
+  yield; yield; let x ← get; yield; set (x + 1); yield;
+
+  let x' ← get; yield; assert (x' = 2); yield;
+  return x'
+
+
+/-- error: Evaluation failed: assertion failed -/
+#guard_msgs in
+#eval evalN raceM 20000 test_race
+
+/-- info: some 1 -/
+#guard_msgs in
+#eval evalN raceM 20000 test_race_ok
+
+/-- info: some 2 -/
+#guard_msgs in
+#eval evalN raceM 20000 test_race_ok2
